verify bigger example

theories/asm.v
@@ -246,26 +246,67 @@ Proof.
   - erewrite map_difference_eq_dom_L => //. apply _.
 Qed.
 
+(** * tsim *)
+Global Hint Transparent asm_instr : tsim.
+Lemma asm_step_WriteReg_i r f es rs ins:
+  TSimStepI asm_module (AsmState (Some (WriteReg r f::es)) rs ins)
+            (λ G, is_Some (rs !! r) ∧ G None (AsmState (Some (es)) (<[r:=f rs]>rs) ins)).
+Proof. constructor => ???????. destruct_and!. invert_all @m_step. naive_solver. Qed.
+Global Hint Resolve asm_step_WriteReg_i : tsim.
+
+Lemma asm_step_Jump_i rs ins:
+  TSimStepI asm_module (AsmState (Some []) rs ins) (λ G,
+    ∀ pc, rs !! "PC" = Some pc →
+          if ins !! pc is Some i then
+            G None (AsmState (Some i) (rs) ins)
+          else
+            G (Some (EJump pc rs)) (AsmState None (rs) ins)
+   ).
+Proof.
+  constructor => ?????? HG. invert_all @m_step; specialize (HG _ ltac:(done)); simplify_option_eq.
+  all: naive_solver.
+Qed.
+Global Hint Resolve asm_step_Jump_i : tsim.
+
+Lemma asm_step_None_i rs ins:
+  TSimStepI asm_module (AsmState None rs ins) (λ G,
+    ∀ pc i rs', rs' !! "PC" = Some pc →
+      ins !! pc = Some i →
+      G (Some (ERecvJump pc rs')) (AsmState (Some i) rs' ins)
+   ).
+Proof. constructor => ?????? HG. invert_all @m_step. naive_solver. Qed.
+Global Hint Resolve asm_step_None_i : tsim.
+
 Require refframe.itree.
 Module asm_examples.
   Import refframe.itree.
   Local Open Scope Z_scope.
   Definition asm_mul : gmap Z asm_instr :=
     <[ 100 := [
-          WriteReg "R3" (λ rs, rs !!! "R1" * rs !!! "R2");
+          (* mul R1, R1, R2 *)
+          WriteReg "R1" (λ rs, rs !!! "R1" * rs !!! "R2");
           WriteReg "PC" (λ rs, rs !!! "PC" + 4)
       ] ]> $
     <[ 104 := [
-          (* Dummy instruction such that we have two instructions *)
-          WriteReg "PC" (λ rs, rs !!! "PC" + 4)
+          (* ret *)
+          WriteReg "PC" (λ rs, rs !!! "R30")
       ] ]> $ ∅.
 
+  (* For supporting recursion, we probably want to be able to
+  non-deterministically break out of the loop. Breaking out at the top
+  level would cause UB (or NB?) but it would be useful for the
+  recursive call *)
   Definition itree_mul : itree (moduleE asm_event unit) unit :=
     ITree.forever (
        pc ← TExist Z;;;
        rs ← TExist _;;;
        TVis (ERecvJump pc rs);;;;
        if bool_decide (pc = 100) then
+         r1 ← TAssumeOpt (rs !! "R1");;;
+         r2 ← TAssumeOpt (rs !! "R2");;;
+         r30 ← TAssumeOpt (rs !! "R30");;;
+         TAssume (r30 ≠ 100 ∧ r30 ≠ 104);;;;
+         TVis (EJump r30 (<["PC":=r30]> $ <["R1":=r1 * r2]> $ rs));;;;
          Ret ()
        else if bool_decide (pc = 104) then
          TUb
@@ -277,20 +318,214 @@ Module asm_examples.
   Lemma asm_mul_refines_itree :
     trefines (MS asm_module (initial_asm_state asm_mul)) (MS (mod_itree _ _) (itree_mul, tt)).
   Proof.
-    apply wp_implies_refines => n /=. rewrite /initial_asm_state.
-    move: (∅) => rs.
-    elim/ti_lt_ind: n rs => n Hloop rs.
-    apply Wp_step => ?????. invert_all @m_step.
-    apply: itree_rel_intro. rewrite /itree_mul unfold_forever !bind_bind.
-    rewrite {1}bind_trigger. eapply thas_trace_Exist.
-    rewrite !bind_bind {1}bind_trigger. eapply thas_trace_Exist.
-    rewrite !bind_bind {1}bind_trigger. eapply thas_trace_Vis.
-    revert select (asm_mul !! _ = Some _) => /lookup_insert_Some[[??]|[? /lookup_insert_Some[[??]|[?/(lookup_empty_Some _ _) ?//]]]]; simplify_eq.
-    2: {
-      rewrite bool_decide_false // bool_decide_true //.
-      rewrite !bind_bind {1}bind_trigger. by eapply thas_trace_All.
-    }
-    rewrite bool_decide_true //.
-  Admitted.
+    apply tsim_implies_trefines => /=. rewrite /initial_asm_state. move: (∅) => rs.
+    move: rs. apply tsim_remember_all => rs.
+    tsim_step_i => pc i rs' HPC Hi.
+    rewrite {1}/itree_mul. rewrite unfold_forever. rewrite -/itree_mul.
 
+    tsim_step_s.
+    tsim_step_s. eexists _.
+    tsim_step_s.
+    tsim_step_s. eexists _.
+    tsim_step_s.
+    tsim_step_s. split; [done|].
+    move: Hi. rewrite !lookup_insert_Some !lookup_empty => Hi. destruct_all!; simplify_eq.
+    all: repeat (rewrite bool_decide_false; [done|]); rewrite bool_decide_true //.
+    all: try by tsim_step_s.
+    tsim_step_s. tsim_step_s => r1 HR1.
+    tsim_step_s. tsim_step_s => r2 HR2.
+    tsim_step_s. tsim_step_s => r30 HR30.
+    tsim_step_s. tsim_step_s => -[??].
+    tsim_step_i. split. { by simplify_map_eq. }
+    erewrite lookup_total_correct; [|done]. erewrite lookup_total_correct; [|done].
+    tsim_step_i. split. { by simplify_map_eq. }
+    erewrite lookup_total_correct; [|by simplify_map_eq].
+    tsim_step_i => ??. simplify_map_eq.
+    tsim_step_i. split. { by simplify_map_eq. }
+    erewrite lookup_total_correct; [|by simplify_map_eq].
+    tsim_step_i => ??. rewrite {1}/asm_mul. simplify_map_eq.
+    tsim_step_s. tsim_step_s. split. { by rewrite insert_insert. }
+    tsim_step_s. tsim_step_s.
+    rewrite -/itree_mul. apply tsim_close_loop. left. naive_solver.
+  Qed.
+
+  Definition asm_mul_client : gmap Z asm_instr :=
+    <[ 200 := [
+          (* mov R1, 2; mov R2, 2; *)
+          WriteReg "R1" (λ rs, 2);
+          WriteReg "R2" (λ rs, 2);
+          WriteReg "PC" (λ rs, rs !!! "PC" + 4)
+      ] ]> $
+    <[ 204 := [
+          (* mov R29, R30; *)
+          WriteReg "R29" (λ rs, rs !!! "R30");
+          WriteReg "PC" (λ rs, rs !!! "PC" + 4)
+      ] ]> $
+    <[ 208 := [
+          (* bl 100; *)
+          WriteReg "R30" (λ rs, rs !!! "PC" + 4);
+          WriteReg "PC" (λ rs, 100)
+      ] ]> $
+    <[ 212 := [
+          (* mov R30, R29; *)
+          WriteReg "R30" (λ rs, rs !!! "R29");
+          WriteReg "PC" (λ rs, rs !!! "PC" + 4)
+      ] ]> $
+    <[ 216 := [
+          (* ret; *)
+          WriteReg "PC" (λ rs, rs !!! "R30")
+      ] ]> $ ∅.
+
+  Definition itree_mul_client : itree (moduleE asm_event unit) unit :=
+    (rec-fix f _ :=
+       b ← translate (inr_) (TAll bool);;;
+       if b then Ret ()
+       else
+       pc ← translate (inr_) (TExist Z);;;
+       rs ← translate (inr_) (TExist _);;;
+       translate (inr_) (TVis (ERecvJump pc rs));;;;
+       if bool_decide (pc = 200) then
+         translate (inr_) (TAssume (is_Some (rs !! "R1")));;;;
+         translate (inr_) (TAssume (is_Some (rs !! "R2")));;;;
+         translate (inr_) (TAssume (is_Some (rs !! "R29")));;;;
+         r30 ← translate (inr_) (TAssumeOpt (rs !! "R30"));;;
+         r29' ← translate (inr_) (TExist Z);;;
+         translate (inr_) (TVis (EJump 100 (<["PC":=100]> $ <["R30":= 212]> $ <["R29":= r29']> $ <["R2":= 2]> $ <["R1":= 2]> $ rs)));;;;
+         f ();;;;
+         pc' ← translate (inr_) (TExist Z);;;
+         rs' ← translate (inr_) (TExist _);;;
+         translate (inr_) (TVis (ERecvJump pc' rs'));;;;
+         translate (inr_) (TAssume (pc' = 212));;;;
+         translate (inr_) (TAssume (is_Some (rs' !! "R30")));;;;
+         translate (inr_) (TAssume (rs' !! "R29" = Some r29'));;;;
+         translate (inr_) (TAssume (r30 ≠ 200 ∧ r30 ≠ 204 ∧ r30 ≠ 208 ∧ r30 ≠ 212 ∧ r30 ≠ 216));;;;
+         r30' ← translate (inr_) (TExist Z);;;
+         translate (inr_) (TVis (EJump r30 (<["PC":= r30]> $ <["R30":= r30']> rs')));;;;
+         f ()
+       else if bool_decide (pc = 204) then translate (inr_) TUb
+       else if bool_decide (pc = 208) then translate (inr_) TUb
+       else if bool_decide (pc = 212) then translate (inr_) TUb
+       else if bool_decide (pc = 216) then translate (inr_) TUb
+       else translate (inr_) TNb
+    ) ();;;; TUb.
+
+    Lemma itree_step_recursive_bind_s EV S R Q A B (f : A → itree (callE A B +' _) _) (t : itree (moduleE EV S) R) (k : R → itree (_ +' moduleE EV S) Q) h s κs:
+      TSimStepS (mod_itree EV S) (x ← interp (recursive f) (ITree.bind (translate inr_ t) k);;; h x, s) κs
+            (λ G, G κs ((ITree.bind t (fun r => x ← interp (recursive f) (k r);;; h x)), s)).
+    Proof.
+      constructor => ????. eexists tnil, _. split; [done|].
+      apply itree_rel_intro. rewrite interp_bind bind_bind interp_translate /= interp_trigger_h.
+      tend => ? <-. done.
+    Qed.
+    Global Hint Resolve itree_step_recursive_bind_s : tsim.
+    Lemma itree_step_recursive_s EV S R A B (f : A → itree (callE A B +' _) _) (t : itree (moduleE EV S) R) h s κs:
+      TSimStepS (mod_itree EV S) (x ← interp (recursive f) (translate inr_ t);;; h x, s) κs
+            (λ G, G κs ((x ← t;;; h x), s)).
+    Proof.
+      constructor => ????. eexists tnil, _. split; [done|].
+      apply itree_rel_intro. rewrite interp_translate /= interp_trigger_h.
+      tend => ? <- /=. done.
+    Qed.
+    Global Hint Resolve itree_step_recursive_s : tsim.
+    Lemma itree_step_interp_ret_s EV S R E  (f : E ~> itree (moduleE EV S)) (a : R) h s κs:
+      TSimStepS (mod_itree EV S) (x ← interp f (Ret a);;; h x, s) κs (λ G, G κs (h a, s)).
+    Proof.
+      constructor => ????. eexists tnil, _. split; [done|].
+      apply itree_rel_intro. rewrite interp_ret bind_ret_l. tend => ? <-. done.
+    Qed.
+    Global Hint Resolve itree_step_interp_ret_s : tsim.
+
+  Lemma tsim_remember_rec {EV S A B} {mi : module EV} σi r (h : B → _) Is s:
+    (∀ x y, tsim mi (mod_itree EV S) (σi x) tnil (h y, s x) Is) →
+    (∀ x h',
+       (∀ x y, tsim mi (mod_itree EV S) (σi x) tnil (h' y, (s x)) Is) →
+       tsim mi (mod_itree EV S) (σi x) tnil ((y ← rec r ();;; h' y), (s x))
+       ((false, λ σ, ∃ x h',
+          σ = (σi x, ((y ← rec r ();;; h' y), s x)) ∧
+          ∀ x y, tsim mi (mod_itree EV S) (σi x) tnil (h' y, s x) Is)::Is)) →
+    ∀ x : A, tsim mi (mod_itree EV S) (σi x) tnil ((y ← rec r ();;; h y), s x) Is.
+  Proof.
+    move => Hh Hsim x.
+    eapply (tsim_remember (ms:=mod_itree _ _)
+      (λ σ, ∃ x h', σ = (σi x, ((y ← rec r ();;; h' y), s x)) ∧
+          ∀ x y, tsim mi (mod_itree EV S) (σi x) tnil (h' y, s x) Is)). { naive_solver. }
+    move => ?? [?[?[[??]?]]]. subst.
+    by apply: Hsim.
+  Qed.
+
+  Lemma tsim_drop_loop {EV} {mi ms : module EV} σi σs κs Is :
+    tsim mi ms σi κs σs [] →
+    tsim mi ms σi κs σs Is.
+  Proof. move => Hsim κs' n _. by apply: Hsim. Qed.
+
+  Lemma asm_mul_client_refines_itree :
+    trefines (MS asm_module (initial_asm_state asm_mul_client)) (MS (mod_itree _ _) (itree_mul_client, tt)).
+  Proof.
+    apply tsim_implies_trefines => /=. rewrite /initial_asm_state. move: (∅) => rs.
+    rewrite {1}/itree_mul_client /rec_fix. set rc := (X in (rec X)).
+    move: rs. apply tsim_remember_rec. { move => ??. rewrite -(bind_ret_r TUb). by tsim_step_s. }
+    move => rs CONT HCONT.
+    rewrite {1}rec_as_interp {2}/rc.
+    tsim_step_s. tsim_step_s => -[].
+    { tsim_step_s. apply: tsim_drop_loop. apply: HCONT. }
+    tsim_step_i => pc i rs' HPC Hi.
+    tsim_step_s. tsim_step_s. eexists _.
+    tsim_step_s. tsim_step_s. eexists _.
+    tsim_step_s. tsim_step_s. split; [done|].
+    move: Hi. rewrite !lookup_insert_Some !lookup_empty => Hi. destruct_all!; simplify_eq.
+    all: repeat (rewrite bool_decide_false; [done|]); rewrite bool_decide_true //.
+    all: try by tsim_step_s; tsim_step_s.
+
+    tsim_step_s. tsim_step_s => -[r1 HR1].
+    tsim_step_s. tsim_step_s => -[r2 HR2].
+    tsim_step_s. tsim_step_s => -[r29 HR29].
+    tsim_step_s. tsim_step_s => r30 HR30.
+    tsim_step_i. split; [ by simplify_map_eq|].
+    tsim_step_i. split; [ by simplify_map_eq|].
+    tsim_step_i. split; [ by simplify_map_eq|].
+    erewrite lookup_total_correct; [|by simplify_map_eq].
+    tsim_step_i => ??. simplify_map_eq.
+    tsim_step_i. split; [ by simplify_map_eq|].
+    erewrite lookup_total_correct; [|by simplify_map_eq].
+    tsim_step_i. split; [ by simplify_map_eq|].
+    erewrite lookup_total_correct; [|by simplify_map_eq].
+    tsim_step_i => ??. simplify_map_eq.
+    tsim_step_i. split; [ by simplify_map_eq|].
+    erewrite lookup_total_correct; [|by simplify_map_eq].
+    tsim_step_i. split; [ by simplify_map_eq|].
+    rewrite insert_commute // insert_insert (insert_commute _ "PC") // insert_insert.
+    tsim_step_i => ??. simplify_map_eq.
+    tsim_step_s. tsim_step_s. eexists r30.
+    tsim_step_s. tsim_step_s. split. {
+      f_equal. apply map_eq => i. apply option_eq => ?.
+      rewrite !lookup_insert_Some. naive_solver.
+    }
+    (* tsim_step_s. *)
+
+    rewrite interp_bind interp_recursive_call.
+    tsim_step_s. apply tsim_close_loop. left. split; [done|]. eexists _, _. split; [done|].
+    move => rs'' ?.
+    tsim_step_i => pc' i rs''' HPC' Hi'.
+    tsim_step_s. tsim_step_s. eexists _.
+    tsim_step_s. tsim_step_s. eexists _.
+    tsim_step_s. tsim_step_s. split; [done|].
+    tsim_step_s. tsim_step_s => ?.
+    unfold asm_mul_client in Hi'. simplify_map_eq.
+    tsim_step_s. tsim_step_s => -[r30'' HR30''].
+    tsim_step_s. tsim_step_s => ?.
+    tsim_step_s. tsim_step_s => -[?[?[?[??]]]].
+    tsim_step_i. split; [ by simplify_map_eq|].
+    erewrite lookup_total_correct; [|by simplify_map_eq].
+    tsim_step_i. split; [ by simplify_map_eq|].
+    erewrite lookup_total_correct; [|by simplify_map_eq].
+    tsim_step_i => ??. simplify_map_eq.
+    tsim_step_i. split; [ by simplify_map_eq|].
+    erewrite lookup_total_correct; [|by simplify_map_eq].
+    tsim_step_i => ??. rewrite {1}/asm_mul_client. simplify_map_eq.
+    tsim_step_s. tsim_step_s. eexists _.
+    tsim_step_s. tsim_step_s. split. { f_equal. by rewrite insert_insert. }
+
+    rewrite interp_recursive_call.
+    apply tsim_close_loop.
+  Qed.
 End asm_examples.
